Change pfunc_list to pfunc_map.

AbstractDomainImpl/PresburgerPwAff.v
@@ -3,17 +3,17 @@ Require Import PolyAI.SSA.
 Require Export Coq.Sets.Ensembles.
 From Coq Require Import ssreflect ssrfun ssrbool.
 
-Definition gamma_pfunc_list {PFunc: Type} {PI: PFuncImpl PFunc} :=
+Definition gamma_pfunc_map {PFunc: Type} {PI: PFuncImpl PFunc} :=
   fun p r => forall s, in_V (eval_map r s) (eval_pfunc (eval_map p s) (eval_map (pointwise_un_op r VVal))).
 
-Definition le_pfunc_list {PFunc: Type} {PI: PFuncImpl PFunc} :=
+Definition le_pfunc_map {PFunc: Type} {PI: PFuncImpl PFunc} :=
   fun a1 a2 => forall_bin_op a1 a2 le_pfunc.
 
-Definition join_pfunc_list {PFunc: Type} {PI: PFuncImpl PFunc} :=
+Definition join_pfunc_map {PFunc: Type} {PI: PFuncImpl PFunc} :=
   fun p1 p2 => pointwise_bin_op p1 p2 join_pfunc.
 
-Theorem le_pfunc_list_refl {PFunc: Type} {PI: PFuncImpl PFunc} :
-  forall a, le_pfunc_list a a.
+Theorem le_pfunc_map_refl {PFunc: Type} {PI: PFuncImpl PFunc} :
+  forall a, le_pfunc_map a a.
 Proof.
   move => a.
   apply forall_bin_op_spec => v.
@@ -21,19 +21,19 @@ Proof.
     by apply le_V_refl.
 Qed.
 
-Theorem le_pfunc_list_trans {PFunc: Type} {PI: PFuncImpl PFunc} :
-  forall a1 a2 a3, le_pfunc_list a1 a2 -> le_pfunc_list a2 a3 -> le_pfunc_list a1 a3.
+Theorem le_pfunc_map_trans {PFunc: Type} {PI: PFuncImpl PFunc} :
+  forall a1 a2 a3, le_pfunc_map a1 a2 -> le_pfunc_map a2 a3 -> le_pfunc_map a1 a3.
 Proof.
   move => a1 a2 a3.
   rewrite !forall_bin_op_spec => H12 H23 v.
     by apply (le_pfunc_trans _ (eval_map a2 v)).
 Qed.
 
-Theorem gamma_pfunc_list_monotone {PFunc: Type} {PI: PFuncImpl PFunc} :
-  forall a1 a2, le_pfunc_list a1 a2 -> Included RegisterMap (gamma_pfunc_list a1) (gamma_pfunc_list a2).
+Theorem gamma_pfunc_map_monotone {PFunc: Type} {PI: PFuncImpl PFunc} :
+  forall a1 a2, le_pfunc_map a1 a2 -> Included RegisterMap (gamma_pfunc_map a1) (gamma_pfunc_map a2).
 Proof.
   move => a1 a2 Hle.
-  rewrite /le_pfunc_list forall_bin_op_spec /Included /In /gamma_pfunc_list in Hle *.
+  rewrite /le_pfunc_map forall_bin_op_spec /Included /In /gamma_pfunc_map in Hle *.
   move => Hle x Hin s.
   move: (Hle s).
   rewrite le_pfunc_spec => Htemp.
@@ -42,45 +42,45 @@ Proof.
   by apply (Htemp2 (eval_map x s)).
 Qed.
 
-Theorem gamma_pfunc_list_top {PFunc: Type} {PI: PFuncImpl PFunc} :
-  forall x, Ensembles.In RegisterMap (gamma_pfunc_list (_ !-> constant_pfunc VTop)) x.
+Theorem gamma_pfunc_map_top {PFunc: Type} {PI: PFuncImpl PFunc} :
+  forall x, Ensembles.In RegisterMap (gamma_pfunc_map (_ !-> constant_pfunc VTop)) x.
 Proof.
   move => x.
-  rewrite /In /gamma_pfunc_list => s.
+  rewrite /In /gamma_pfunc_map => s.
     by simpl_pfunc.
 Qed.
 
-Theorem join_pfunc_list_sound_l {PFunc: Type} {PI: PFuncImpl PFunc} :
-  forall a1 a2, le_pfunc_list a1 (join_pfunc_list a1 a2).
+Theorem join_pfunc_map_sound_l {PFunc: Type} {PI: PFuncImpl PFunc} :
+  forall a1 a2, le_pfunc_map a1 (join_pfunc_map a1 a2).
 Proof.
   move => a1 a2.
-  rewrite /join_pfunc_list /le_pfunc_list forall_bin_op_spec => v.
+  rewrite /join_pfunc_map /le_pfunc_map forall_bin_op_spec => v.
   rewrite pointwise_bin_op_spec.
   apply join_pfunc_spec_l.
 Qed.
 
-Theorem join_pfunc_list_sound_r {PFunc: Type} {PI: PFuncImpl PFunc} :
-  forall a1 a2, le_pfunc_list a2 (join_pfunc_list a1 a2).
+Theorem join_pfunc_map_sound_r {PFunc: Type} {PI: PFuncImpl PFunc} :
+  forall a1 a2, le_pfunc_map a2 (join_pfunc_map a1 a2).
 Proof.
   move => a1 a2.
-  rewrite /join_pfunc_list /le_pfunc_list forall_bin_op_spec => v.
+  rewrite /join_pfunc_map /le_pfunc_map forall_bin_op_spec => v.
   rewrite pointwise_bin_op_spec.
   apply join_pfunc_spec_r.
 Qed.
 
-Instance PFuncListAD {PFunc: Type} (PI: PFuncImpl PFunc) : adom (total_map PFunc) :=
+Instance PFuncMapAD {PFunc: Type} (PI: PFuncImpl PFunc) : adom (total_map PFunc) :=
   {
-    le := le_pfunc_list;
+    le := le_pfunc_map;
     bot := (_ !-> constant_pfunc VBot);
     top := (_ !-> constant_pfunc VTop);
-    join := join_pfunc_list;
+    join := join_pfunc_map;
 
-    gamma := gamma_pfunc_list;
+    gamma := gamma_pfunc_map;
 
-    le_refl := le_pfunc_list_refl;
-    le_trans := le_pfunc_list_trans;
-    gamma_monotone := gamma_pfunc_list_monotone;
-    gamma_top := gamma_pfunc_list_top;
-    join_sound_l := join_pfunc_list_sound_l;
-    join_sound_r := join_pfunc_list_sound_r;
+    le_refl := le_pfunc_map_refl;
+    le_trans := le_pfunc_map_trans;
+    gamma_monotone := gamma_pfunc_map_monotone;
+    gamma_top := gamma_pfunc_map_top;
+    join_sound_l := join_pfunc_map_sound_l;
+    join_sound_r := join_pfunc_map_sound_r;
   }.
